# Problem set 3 solutions

:::{.callout-tip}
## Note
This material has not yet been finalised and is still under construction. Once it is covered in lectures, this banner will be replaced.
:::

$$
\begin{aligned}
\epsilon T'' + 2T' + T &= 0, \\
T(0) &= 0, \\
T(1) &= 1.
\end{aligned}
$$

The challenge is to study the above problem for small values of $\epsilon$. 


## Conversion to first-order system

By using the procedure reviewed in @sec-asym2-num,  convert (@eq-ps3-sys) to a first-order system of equations.

:::{.callout-important collapse=true}
## Solution
Introduce $u(z) = T(z)$ and $v(z) = T'(z)$. Then 
$$
\frac{\mathrm{d}}{\mathrm{d}z}\begin{pmatrix}
u \\
v
\end{pmatrix} =
\begin{pmatrix}
v \\
-\frac{1}{\epsilon} (2v + u)
\end{pmatrix}
$$ 
:::

## Numerical solutions

:::{.callout-important collapse=true}
## Solution
A script can be found in `problemsets/ps03_solutions.ipynb`
:::

## Investigation of the boundary layer

Using your code, use the following command in order to investigate the maxima $(x_m, T_m)$ as $\epsilon$ varies:

	ind = np.argmax(Y[0])
	print(ep, z[ind], Y[0, ind])

You may want to consider, as an example, the values $\epsilon = \{0.05, 0.1, 0.15, 0.2\}$ and fill the following table. 

| $\epsilon$ | $z_m$ | $T_m$ |
| -- | -- | -- |
| 0.05 | 0.1122 | 1.5479 | 
| 0.1 | 0.1924| 1.4742 |
| 0.15 | 0.2605 | 1.4094 | 
| 0.2 | 0.3226  | 1.3501 |

Create a plot of $(\epsilon, x_m)$ and discuss the observed trend and its implications.

:::{.callout-important collapse=true}
## Solution

![A plot of the above data. This looks linear, and indeed this provides numerical confirmation that the boundary layer should be sized with $\epsilon$](img/2023-03-09-11-21-25.png){#fig- width=80%}
:::



## Outer asymptotic solutions

Begin by setting 
$$
T = T_{\text{outer}} = T_0(z) + \epsilon T_1(z) + \epsilon^2 T_2(z) + \ldots
$$ 
Substitute the above expansion into the system and solve for the first two orders. 

You may verify that the solution is given by 

\begin{align}
T_0 &= e^{1/2} e^{-z/2}, \\
T_1 &= -\frac{1}{8} e^{1/2} e^{-z/2} (z - 1).
\end{align}


:::{.callout-important collapse=true}
## Solution
**Remember**: as you solve the outer solution, you impose the boundary condition of $T(1) = 1$.

**Leading-order**: at leading order, we get the problem $2T_0' + T_0 = 0$ subject to $T_0(1) = 1$. This is solved either by separation of variables or by integrating factor. Using the technique of solving first-order linear equations, (see @sec-odes) we divide,
$$
T_0' + \frac{1}{2}T_0 = 0.
$$ 
We then multiply both sides of the equation by $e^{z/2}$. 
$$
\frac{\mathrm{d}}{\mathrm{d}z}\Bigl[T_0 e^{z/2}\Bigr] = 0.
$$ 
Integrate, and solve, giving $T_0 = Ce^{-z/2}$. We now impose $T_0(1) = 1$ which yields $C = e^{1/2}$.

**First-order**: at next order, we get
$$
2T_1' + T_1 = -T_0'' \Longrightarrow T_1' + \frac{1}{2}T_1 = -\frac{1}{2}T_0'' ,
$$ 
along with the boundary conditions of $T_1(1) = 0$. 

Again place this into the appropriate form. Again, this is a linear first-order equation. We multiply by the integrating factor $e^{z/2}$, placing the equation into the form 
$$
\frac{\mathrm{d}}{\mathrm{d}z} \Bigl[ T_1 e^{z/2} \Bigr] = -\frac{1}{2 }T_0'' e^{z/2} = -\frac{1}{8} e^{1/2}.
$$ 
We integrate once and simplify, yielding
$$
T_1(z) = \left(-\frac{e^{1/2}}{8} z + C\right)e^{-z/2},
$$ 
and then impose the condition that $T_1(1) = 0$. This yields $C = e^{1/2}/8$ hence
$$
T_1(z) = -\frac{e^{1/2}}{8}(z - 1) e^{-z/2}.
$$ 
:::


## Inner asymptotic solutions

There will be a boundary layer near $z = 0$. Set $z = \epsilon^{\alpha} s$ and $T(z) = U(s)$. Follow the same procedure, as in @sec-asymptotics03 in order to determine the correct choice of $\alpha$ for the inner region. This choice should balance the two terms $\epsilon T''$ and $2T'$. 

:::{.callout-important collapse=true}
## Solution
We re-scale $z = \epsilon^\alpha s$ and let $T(s) = U(s)$. Then the ODE becomes
$$
\epsilon^{1 - 2\alpha} U'' + 2 \epsilon^{-\alpha} U' + U = 0.
$$ 
Balancing the first two terms thus requires that 
$$
1 - 2 \alpha = -\alpha \Longrightarrow \alpha = 1.
$$ 
Thus the differential equation now becomes 
$$
U'' + 2 U' + \epsilon U = 0.
$$ 
:::

## Matching and comparison

Expanding the inner solution as $U = U_0(s) + \epsilon U_1(s) + \ldots$, write down the equation and boundary conditions that $U_0$ must satisfy. You will notice that $U_0$ is governed by a second-order differential equation and therefore needs two boundary conditions. One boundary condition comes from $z = 0$, i.e.
$$
U_0(0) = 0.
$$ 

The other boundary condition is a matching condition:
$$
\lim_{s \to \infty} U_0(s) = \lim_{z \to 0} T_0(z),
$$ 
which imposes that the inner solution, as it leaves the boundary layer, matches the outer solution, it tends into the inner region.

:::{.callout-important collapse=true}
## Solution
Solve for $U_0$.

We thus expand $U = U_0 + \epsilon U_1 + \ldots$. To leading order, we have 
$$
U_0'' + 2U_0' = 0.
$$ 
Integrating, we find that the general solution is given by 
$$
U_0(s) = C_1 + C_2 e^{-2s}.
$$ 
We require two boundary conditions. The first condition is given by $T(0) = 0$ and hence $U(0) = 0$. The second condition is given by requiring that the inner solution, as $s \to \infty$, matches the outer solution, as $z \to 0$. Using our solution above, we find that 
$$
\lim_{z \to 0} T_0(z) = e^{1/2}. 
$$ 
Thus the second boundary condition is 
$$
\lim_{s \to \infty} U_0(s) = e^{1/2}.
$$ 
Together, both boundary conditions are used to conclude that 
$$
U_0(s) = e^{1/2}(1 - e^{-2s}),
$$ 
or in terms of $z$, the inner solution is 
$$
T_{\text{inner}} \sim e^{1/2}(1 - e^{-2z/\epsilon}).
$$ 
:::
 


